while example

proofs.v
@@ -35,3 +35,67 @@ Proof.
     eapply BigStepTrans;[constructor|apply BigStepEnd].
     intros [c H];inversion H.
 Qed.
+
+Import String.
+Open Scope string.
+
+Variable (S:Stmt).
+
+Definition wp := Block
+    [
+        While (Binary Ge (LVal (Var "a")%string) (LVal(Var "b")%string))
+        (* extra Block in Exercise *)
+                (Assign (Var "a")%string (Binary Sub (LVal (Var "a")%string) (LVal (Var "b")%string)))
+        ; S
+    ].
+
+    Print State.
+    Print VarEnv.
+    Print MemEnv.
+(* Definition △ := 0. *)
+Instance eqString : EqDec string.
+constructor.
+repeat decide equality.
+Defined.
+
+
+Definition ρ : VarEnv :=
+    update
+    (update (fun _ => None) "a" (Some 0))
+    "b" (Some 1)
+    . 
+Definition μ : MemEnv :=
+    update
+    (update (fun _ => None) 0 (Some (Defined 42)))
+    1 (Some (Defined 17))
+    . 
+
+
+Definition σ := (ρ,μ).
+
+Goal exists T, ⟨ wp | σ ⟩ ⇓ T.
+Proof.
+eexists.
+unfold wp.
+eapply BigStepTrans.
+ 1: {
+    apply SubstStep.
+    apply WhileStep.
+ }
+eapply BigStepTrans.
+ 1: {
+    apply SubstStep.
+    apply IfTrueStep with (n:=1).
+    all:admit.
+ }
+eapply BigStepTrans.
+ 1: {
+    (* apply ExecStep. *)
+    apply SubstStep. (* Not Exec as exec is going to <s,sig> not Terminal *)
+    apply ExecStep.
+    (* apply AssignStep. *)
+    admit.
+ }
+eapply BigStepTrans.
+ 1: {
+    apply ExecStep.
